src/goose_lang/ffi/grove_ffi.v
@@ -1,5 +1,5 @@
 From Perennial.goose_lang Require Import prelude.
-From Perennial.goose_lang Require Import ffi.disk_prelude.
+From Perennial.goose_lang Require Export ffi.disk_prelude.
 
 Axiom Read : val.
 Axiom Write : val.
