src/goose_lang/ffi/grove_prelude.v
@@ -1,0 +1,2 @@
+From Perennial.goose_lang Require Import prelude.
+From Perennial.goose_lang Require ffi.grove_ffi.
